src/db/type.lean
@@ -13,4 +13,16 @@ inductive db : ℕ → Type
   | app : Π {n : ℕ}, db n → db n → db n  -- application
   | lam : Π {n : ℕ}, db (succ n) → db n  -- lambda abstraction
 
+namespace db -------------------------------------------------------------------
+
+def repr : ∀ {n : ℕ}, db n → string
+  | n (var N)   := _root_.repr N
+  | n (app f e) := "(" ++ repr f ++ " " ++ repr e ++ ")"
+  | n (lam e)   := "(λ " ++ repr e ++ ")"
+
+instance has_repr (n : ℕ) : has_repr (db n) :=
+  ⟨@repr n⟩
+
+end /- namespace -/ db ---------------------------------------------------------
+
 end /- namespace -/ acie -------------------------------------------------------
